Ftlr load case: refactoring using lemma's
Introduced the major lemma's used in the body of the load case
Rewrote parts within these lemma's using smaller auxiliary lemma's from rules_base

theories/ftlr/Load.v
@@ -32,9 +32,22 @@ Section fundamental.
        else ▷ monotonicity_guarantees_region ρ v p φ ∗  ▷ φ (W, v) )
     ∗ rel l p φ)%I.
 
+  Lemma load_inr_eq {regs r p0 g0 b0 e0 a0 p1 g1 b1 e1 a1}:
+    reg_allows_load regs r p0 g0 b0 e0 a0 →
+    read_reg_inr regs r p1 g1 b1 e1 a1 →
+    p0 = p1 ∧ g0 = g1 ∧ b0 = b1 ∧ e0 = e1 ∧ a0 = a1.
+  Proof.
+      intros Hrar H3.
+      pose (Hrar' := Hrar).
+      destruct Hrar' as (Hinr0 & _ & _). destruct H3 as [Hinr1 | Hinl1].
+      * rewrite Hinr0 in Hinr1. inversion Hinr1.
+        rewrite H4 H5 H6 H7 H8 in Hrar; auto.
+      * destruct Hinl1 as [z Hinl1]. rewrite Hinl1 in Hinr0. by exfalso.
+  Qed. 
+
 
   (* Description of what the resources are supposed to look like after opening the region if we need to, but before closing the region up again*)
-  Definition allow_load_res_or_true W r (regs : Reg) pc_a pc_p:=
+  Definition allow_load_res W r (regs : Reg) pc_a pc_p:=
     (∃ p g b e a, ⌜read_reg_inr regs r p g b e a⌝ ∗
     if decide (reg_allows_load regs r p g b e a ) then
        if decide (a ≠ pc_a) then
@@ -42,13 +55,199 @@ Section fundamental.
        else ⌜PermFlows p pc_p⌝ ∗ open_region pc_a W
       else open_region pc_a W)%I.
 
-  Definition allow_load_mem_or_true W r (regs : Reg) pc_a pc_p pc_w (mem : PermMem) (bl: bool):=
+  Definition allow_load_mem W r (regs : Reg) pc_a pc_p pc_w (mem : PermMem) (bl: bool):=
     (∃ p g b e a, ⌜read_reg_inr regs r p g b e a⌝ ∗
     if decide (reg_allows_load regs r p g b e a) then
        if decide (a ≠ pc_a) then
          ∃ p' w, ⌜mem = <[a:=(p',w)]> (<[pc_a:=(pc_p,pc_w)]> ∅)⌝ ∗
             ⌜PermFlows p p'⌝ ∗ (region_open_resources W a [pc_a] p' interpC w bl)
        else  ⌜mem = <[pc_a:=(pc_p,pc_w)]> ∅⌝ ∗ ⌜PermFlows p pc_p⌝ ∗ open_region pc_a W     else  ⌜mem = <[pc_a:=(pc_p,pc_w)]> ∅⌝ ∗ open_region pc_a W)%I.
+
+  Lemma create_load_res:
+    ∀ (W : leibnizO (STS * STS)) (r : leibnizO Reg) (p p' : Perm)
+      (g : Locality) (b e a : Addr) (src : RegName) (p0 : Perm)
+      (g0 : Locality) (b0 e0 a0 : Addr),
+      PermFlows p p'
+      → read_reg_inr (<[PC:=inr (p, g, b, e, a)]> r) src p0 g0 b0 e0 a0
+      → (∀ r1 : RegName, ⌜r1 ≠ PC⌝ → ((fixpoint interp1) W) (r !r! r1))
+          -∗ read_write_cond a p' interp
+          -∗ open_region a W
+          -∗ sts_full_world sts_std W
+          -∗ allow_load_res W src (<[PC:=inr (p, g, b, e, a)]> r) a p'
+          ∗ sts_full_world sts_std W.
+  Proof.
+    intros W r p p' g b e a src p0 g0 b0 e0 a0 Hpf HVsrc.
+    iIntros "#Hreg #Hinva Hr Hsts".
+    do 5 (iApply sep_exist_r; iExists _). iFrame "%".
+    destruct (decide (reg_allows_load (<[PC:=inr (p, g, b, e, a)]> r) src p0 g0 b0 e0 a0)). 1: rename r0 into Hallows.
+    -  destruct Hallows as [Hrinr [Hra Hwb] ].
+       destruct (decide (a0 ≠ a)); rename n into Haeq.
+       * apply andb_prop in Hwb as [Hle Hge].
+         rewrite /leb_addr in Hle,Hge.
+
+         (* Unlike in the old proof, we now go the other way around, and prove that the source register could not have been the PC, since both addresses differ. This saves us some cases.*)
+         assert (src ≠ PC) as n.
+         {
+           intros contra. rewrite contra in Hrinr.
+           rewrite lookup_insert in Hrinr. inversion Hrinr. congruence.
+         }
+
+         iDestruct ("Hreg" $! src n) as "Hvsrc".
+         rewrite lookup_insert_ne in Hrinr; last by congruence.
+         rewrite /RegLocate Hrinr.
+         iDestruct (read_allowed_inv _ a0 with "Hvsrc") as "Hconds"; auto;
+           first (split; [by apply Z.leb_le | by apply Z.ltb_lt]).
+
+         rewrite /read_write_cond.
+         iDestruct "Hconds" as (p0' Hfl') "Hrel'".
+         iDestruct (region_open_prepare with "Hr") as "Hr".
+         iDestruct (readAllowed_valid_cap_implies with "Hvsrc") as "%"; eauto.
+         { rewrite /withinBounds /leb_addr Hle Hge. auto. }
+         destruct H3 as [Hregion' [ρ' [Hstd' Hnotrevoked'] ] ].
+         (*We can finally frame off Hsts here, since it is no longer needed after opening the region*)
+         iDestruct (region_open_next _ _ _ a0 p0' ρ' with "[$Hrel' $Hr $Hsts]") as (w0) "($ & Hstate' & Hr & Ha0 & % & Hfuture & #Hval)"; eauto.
+         { apply not_elem_of_cons. split; auto. apply not_elem_of_nil. }
+         iExists p0', w0. iSplitL "Ha0"; auto. iSplitR; auto. unfold region_open_resources.
+         iExists ρ'. iFrame "%". iFrame. by iFrame "#".
+       * iFrame.
+         destruct (decide (src = PC)) ; simplify_eq.
+          + rewrite lookup_insert in Hrinr.
+            inversion Hrinr. rewrite -H4. auto.
+          +  iDestruct ("Hreg" $! src n) as "Hsrcv".
+              rewrite lookup_insert_ne in Hrinr; last by congruence.
+              rewrite /RegLocate Hrinr.
+              iDestruct (read_allowed_inv _ a0 with "Hsrcv") as (p'' Hfl') "#Harel'".
+              { apply andb_true_iff in Hwb as [Hle Hge].
+                split; [by apply Z.leb_le | by apply Z.ltb_lt]; auto. }
+              { destruct p0; inversion Hra; auto. }
+              rewrite /read_write_cond.
+              assert (a0 = a). by apply dec_stable.
+              rewrite -H3.
+                by iDestruct (rel_agree a0 p' p'' with "[$Hinva $Harel']") as "[-> _]".
+    - iFrame.
+  Qed.
+
+  Lemma load_res_implies_mem_map:
+    ∀ (W : leibnizO (STS * STS)) (r : leibnizO Reg) (p p' : Perm)
+      (g : Locality) (b e a : Addr) (w : Word) (src : RegName),
+      allow_load_res W src (<[PC:=inr (p, g, b, e, a)]> r) a p'
+      -∗ a ↦ₐ[p'] w
+      -∗ ∃ mem0 : PermMem,
+          allow_load_mem W src (<[PC:=inr (p, g, b, e, a)]> r) a p' w mem0 false
+            ∗ ▷ ([∗ map] a0↦pw ∈ mem0, ∃ (p0 : Perm) (w0 : leibnizO Word),
+                ⌜pw = (p0, w0)⌝ ∗ a0 ↦ₐ[p0] w0).
+  Proof.
+    intros W r p p' g b e a w src.
+    iIntros "HLoadRes Ha".
+    iDestruct "HLoadRes" as (p1 g1 b1 e1 a1) "[% HLoadRes]".
+
+    case_decide as Hallows.
+    -  pose(Hallows' := Hallows). destruct Hallows' as [Hrinr [Hra Hwb] ].
+        case_decide as Haeq.
+        * iDestruct "HLoadRes" as (p'0 w0) "[HLoadCh HLoadRest]".
+          iExists _.
+          iSplitL "HLoadRest".
+          + iExists p1,g1,b1,e1,a1. iSplitR; first auto.
+            do 2 (case_decide; last by exfalso).
+            iExists p'0,w0. iSplitR; auto.
+          + iNext.
+            iApply memMap_resource_2ne; auto; iFrame.
+      * iExists _.
+        iSplitL "HLoadRes".
+          + iExists p1,g1,b1,e1,a1. iSplitR; auto.
+            case_decide; last by exfalso. case_decide; first by exfalso.
+            iDestruct "HLoadRes" as (HPF) "HLoadRes". iSplitR; auto.
+          + iNext. by iApply memMap_resource_1.
+    - iExists _.
+      iSplitL "HLoadRes".
+      + iExists p1,g1,b1,e1,a1. iSplitR; auto.
+        case_decide; first by exfalso. auto.
+      + iNext. by iApply memMap_resource_1.
+    Qed.
+
+  Lemma mem_map_implies_pure_conds:
+    ∀ (W : leibnizO (STS * STS)) (r : leibnizO Reg) (p p' : Perm)
+      (g : Locality) (b e a : Addr) (w : Word) (src : RegName)
+      (mem0 : PermMem),
+        allow_load_mem W src (<[PC:=inr (p, g, b, e, a)]> r) a p' w mem0 false
+        -∗ ⌜mem0 !! a = Some (p', w)⌝
+          ∗ ⌜allow_load_map_or_true src (<[PC:=inr (p, g, b, e, a)]> r) mem0⌝.
+  Proof.
+    iIntros (W r p p' g b e a w src mem0) "HLoadMem".
+    iDestruct "HLoadMem" as (p1 g1 b1 e1 a1) "[% HLoadRes]".
+    case_decide as Hallows.
+    -  pose(Hallows' := Hallows). destruct Hallows' as [Hrinr [Hra Hwb] ].
+        case_decide as Haeq.
+        * iDestruct "HLoadRes" as (p'0 w0 ->) "[% _]".
+          iSplitR. rewrite lookup_insert_ne; auto. by rewrite lookup_insert.
+          iExists p1,g1,b1,e1,a1. iSplitR; auto.
+          case_decide; last by exfalso.
+          iExists p'0,w0. iSplitR; auto.
+          by rewrite lookup_insert.
+        * iDestruct "HLoadRes" as "[-> [% HLoadRes] ]".
+          iSplitR. by rewrite lookup_insert.
+          iExists p1,g1,b1,e1,a1. iSplitR; auto.
+          case_decide; last by exfalso.
+          iExists p',w. by rewrite Haeq lookup_insert.
+    - iDestruct "HLoadRes" as "[-> HLoadRes]".
+      iSplitR. by rewrite lookup_insert.
+      iExists p1,g1,b1,e1,a1. iSplitR; auto.
+      case_decide; first by exfalso. auto.
+  Qed.
+
+  Lemma allow_load_mem_later:
+    ∀ (W : leibnizO (STS * STS)) (r : leibnizO Reg) (p p' : Perm)
+      (g : Locality) (b e a : Addr) (w : Word) (src : RegName)
+      (mem0 : PermMem),
+      allow_load_mem W src (<[PC:=inr (p, g, b, e, a)]> r) a p' w mem0 false
+      -∗ ▷ allow_load_mem W src (<[PC:=inr (p, g, b, e, a)]> r) a p' w mem0 true.
+  Proof.
+    iIntros (W r p p' g b e a w src mem0) "HLoadMem".
+    iDestruct "HLoadMem" as (p0 g0 b0 e0 a0) "[% HLoadMem]".
+    do 5 (iApply later_exist_2; iExists _). iApply later_sep_2; iSplitR; auto.
+    case_decide.
+    - case_decide.
+      * iDestruct "HLoadMem" as (p'0 w0) "[-> [% HLoadMem] ]".
+        do 2 (iApply later_exist_2; iExists _).
+        do 2 (iApply later_sep_2; iSplitR; auto).
+      * iFrame.
+    - iFrame.
+  Qed.
+
+  Lemma mem_map_recover_res:
+    ∀ (W : leibnizO (STS * STS)) (r : leibnizO Reg) (p p' : Perm)
+      (g : Locality) (b e a : Addr) (w : Word) (src : RegName)  (p0 p'0 : Perm)
+      (g0 : Locality) (b0 e0 a0 : Addr) (mem0 : PermMem) (loadv : Word),
+      reg_allows_load (<[PC:=inr (p, g, b, e, a)]> r) src p0 g0 b0 e0 a0
+      → mem0 !! a0 = Some (p'0, loadv)
+      → allow_load_mem W src (<[PC:=inr (p, g, b, e, a)]> r) a p' w mem0 true
+        -∗ ((fixpoint interp1) W) w
+        -∗ ([∗ map] a0↦pw ∈ mem0, ∃ (p0 : Perm) (w0 : Word),
+                ⌜pw = (p0, w0)⌝ ∗ a0 ↦ₐ[p0] w0)
+        -∗ open_region a W ∗ a ↦ₐ[p'] w ∗ ((fixpoint interp1) W) loadv.
+  Proof.
+    intros W r p p' g b e a w src p0 p'0 g0 b0 e0 a0 mem0 loadv Hrar Ha0.
+    iIntros "HLoadMem #Hw Hmem".
+    iDestruct "HLoadMem" as (p1 g1 b1 e1 a1) "[% HLoadRes]".
+    destruct (decide (reg_allows_load (<[PC:=inr (p, g, b, e, a)]> r) src p1 g1 b1 e1 a1)). 1: rename r0 into Hallows.
+    -  destruct Hallows as [Hrinr [Hra Hwb] ].
+        destruct (decide (a1 ≠ a)); rename n into Haeq.
+        * iDestruct "HLoadRes" as (p'1 w0) "[-> [% HLoadRes] ]".
+          iDestruct "HLoadRes" as (ρ1) "(Hstate' & % & Hr & % & (Hfuture & #HV) & Hrel')".
+          rewrite -memMap_resource_2ne. iDestruct "Hmem" as  "[Ha1 $]".
+          iDestruct (region_close_next with "[$Hr $Ha1 $Hrel' $Hstate' $Hfuture]") as "Hr"; eauto.
+          { apply not_elem_of_cons; split; [auto|apply not_elem_of_nil]. }
+          iDestruct (region_open_prepare with "Hr") as "$".
+          destruct (load_inr_eq Hrar H3) as (<- & <- &<- &<- &<-).
+          rewrite lookup_insert in Ha0; inversion Ha0. all: done.
+        * apply dec_stable in Haeq.
+          iDestruct "HLoadRes" as "[-> [% $ ] ]".
+          rewrite -memMap_resource_1.
+          destruct (load_inr_eq Hrar H3) as (<- & <- &<- &<- &<-).
+          rewrite Haeq lookup_insert in Ha0. inversion Ha0. by iFrame.
+    - destruct (load_inr_eq Hrar H3) as (<- & <- &<- &<- &<-); by exfalso.
+  Qed.
+
 
   Lemma load_case(W : WORLD) (r : leibnizO Reg) (p p' : Perm)
         (g : Locality) (b e a : Addr) (w : Word) (ρ : region_type) (dst src : RegName) :
@@ -61,7 +260,7 @@ Section fundamental.
     iDestruct ((big_sepM_delete _ _ PC) with "[HPC Hmap]") as "Hmap /=";
       [apply lookup_insert|rewrite delete_insert_delete;iFrame|]. simpl.
 
-    (* Handy to read out PC's name later, and needed when calling wp_load *)
+    (* To read out PC's name later, and needed when calling wp_load *)
     assert(∀ x : RegName, is_Some (<[PC:=inr (p, g, b, e, a)]> r !! x)) as Hsome'.
     {
       intros. destruct (decide (x = PC)).
@@ -70,151 +269,27 @@ Section fundamental.
     }
 
     (* Initializing the names for the values of Hsrc now, to instantiate the existentials in step 1*)
-    specialize Hsome' with src as Hsrc.
-    destruct Hsrc as [wsrc Hsomesrc].
     assert (∃ p0 g0 b0 e0 a0 , read_reg_inr (<[PC:=inr (p, g, b, e, a)]> r) src p0 g0 b0 e0 a0) as [p0 [g0 [b0 [e0 [a0 HVsrc] ] ] ] ].
     {
+      specialize Hsome' with src as Hsrc.
+      destruct Hsrc as [wsrc Hsomesrc].
       unfold read_reg_inr. destruct wsrc. 2: destruct c,p0,p0,p0. all: repeat eexists.
-      right. by exists z.
-      by left.
+      right. by exists z. by left.
     }
 
-    (* Step 1: open the region, if necessary, and store all the resources obtained from the region in allow_load_res_or_true *)
-    iAssert (allow_load_res_or_true W src (<[PC:=inr (p, g, b, e, a)]> r) a p' ∗ sts_full_world sts_std W)%I with "[Hr Hsts]" as "[HLoadRes Hsts]".
-    {
-      unfold allow_load_res_or_true.
-      do 5 (iApply sep_exist_r; iExists _). iFrame "%".
-      destruct (decide (reg_allows_load (<[PC:=inr (p, g, b, e, a)]> r) src p0 g0 b0 e0 a0)). 1: rename r0 into Hallows.
-
-      -  destruct Hallows as [Hrinr [Hra Hwb] ].
-         destruct (decide (a0 ≠ a)); rename n into Haeq.
-         * apply andb_prop in Hwb as [Hle Hge].
-           rewrite /leb_addr in Hle,Hge.
-
-           (* Unlike in the old proof, we now go the other way around, and prove that the source register could not have been the PC, since both addresses differ. This saves us some cases.*)
-           assert (src ≠ PC) as n.
-           {
-             intros contra. rewrite contra in Hrinr.
-             rewrite lookup_insert in Hrinr. inversion Hrinr. congruence.
-           }
-
-           iDestruct ("Hreg" $! src n) as "Hvsrc".
-           rewrite lookup_insert_ne in Hrinr; last by congruence.
-           rewrite /RegLocate Hrinr.
-           iDestruct (read_allowed_inv _ a0 with "Hvsrc") as "Hconds"; auto;
-            first (split; [by apply Z.leb_le | by apply Z.ltb_lt]).
-
-          rewrite /read_write_cond.
-          iDestruct "Hconds" as (p0' Hfl') "Hrel'".
-          iDestruct (region_open_prepare with "Hr") as "Hr".
-          iDestruct (readAllowed_valid_cap_implies with "Hvsrc") as "%"; eauto.
-          { rewrite /withinBounds /leb_addr Hle Hge. auto. }
-          destruct H3 as [Hregion' [ρ' [Hstd' Hnotrevoked'] ] ].
-          (*We can finally frame off Hsts here, since it is no longer needed after opening the region*)
-          iDestruct (region_open_next _ _ _ a0 p0' ρ' with "[$Hrel' $Hr $Hsts]") as (w0) "($ & Hstate' & Hr & Ha0 & % & Hfuture & #Hval)"; eauto.
-          { apply not_elem_of_cons. split; auto. apply not_elem_of_nil. }
-          iExists p0', w0. iSplitL "Ha0"; auto. iSplitR; auto. unfold region_open_resources.
-          iExists ρ'. iFrame "%". iFrame. by iFrame "#".
-        * iFrame.
-          destruct (decide (src = PC)) ; simplify_eq.
-          + rewrite lookup_insert in Hrinr.
-            inversion Hrinr. rewrite -H4. auto.
-          +  iDestruct ("Hreg" $! src n) as "Hsrcv".
-             rewrite lookup_insert_ne in Hrinr; last by congruence.
-             rewrite /RegLocate Hrinr.
-             iDestruct (read_allowed_inv _ a0 with "Hsrcv") as (p'' Hfl') "#Harel'".
-             { apply andb_true_iff in Hwb as [Hle Hge].
-               split; [by apply Z.leb_le | by apply Z.ltb_lt]; auto. }
-             { destruct p0; inversion Hra; auto. }
-             rewrite /read_write_cond.
-             assert (a0 = a). by apply dec_stable.
-             rewrite -H3.
-             by iDestruct (rel_agree a0 p' p'' with "[$Hinva $Harel']") as "[-> _]".
-      - iFrame.
-    }
+    (* Step 1: open the region, if necessary, and store all the resources obtained from the region in allow_load_res *)
+    iDestruct (create_load_res with "Hreg Hinva Hr Hsts") as "[HLoadRes Hsts]"; eauto.
     (* Clear helper values; they exist in the existential now *)
     clear HVsrc p0 g0 b0 e0 a0.
 
     (* Step2: derive the concrete map of memory we need, and any spatial predicates holding over it *)
-    iAssert (∃mem, allow_load_mem_or_true W src (<[PC:=inr (p, g, b, e, a)]> r) a p' w mem false ∗ (▷ [∗ map] a↦pw ∈ mem, ∃ p w, ⌜pw = (p,w)⌝ ∗ a ↦ₐ[p] w) )%I with "[HLoadRes Ha]" as (mem) "[HLoadMem HMemRes]".
-    {
-      unfold allow_load_res_or_true. iDestruct "HLoadRes" as (p1 g1 b1 e1 a1) "[% HLoadRes]".
-      unfold allow_load_mem_or_true.
-      iAssert (∃ (p1 : Perm) (w1 : leibnizO Word), ⌜(p',w) = (p1, w1)⌝ ∗ a ↦ₐ[p1] w1)%I with "[Ha]" as "Ha". iExists p',w. auto.
-
-      case_decide as Hallows.
-      -  pose(Hallows' := Hallows). destruct Hallows' as [Hrinr [Hra Hwb] ].
-         case_decide as Haeq.
-         * iDestruct "HLoadRes" as (p'0 w0) "[HLoadCh HLoadRest]".
-           iExists (<[a1:=(p'0, w0)]> (<[a:=(p', w)]> ∅)).
-
-           iSplitL "HLoadRest".
-           + iExists p1,g1,b1,e1,a1. iSplitR; first auto.
-             do 2 (case_decide; last by exfalso).
-             iExists p'0,w0. iSplitR; auto.
-           + iNext.
-             iAssert (∃ (p1 : Perm) (w1 : leibnizO Word), ⌜(p'0,w0) = (p1, w1)⌝ ∗ a1 ↦ₐ[p1] w1)%I with "[HLoadCh]" as "HLoadCh". iExists p'0,w0. by iSplitR.
-
-             rewrite (big_sepM_insert _ _).
-             rewrite (big_sepM_insert _ _).
-             iFrame. rewrite (big_opM_empty). auto.
-             ++ auto.
-             ++ rewrite lookup_insert_ne; auto.
-         * iExists ( <[a:=(p', w)]> ∅).
-           iSplitL "HLoadRes".
-           + iExists p1,g1,b1,e1,a1. iSplitR; auto.
-             case_decide; last by exfalso. case_decide; first by exfalso.
-             iDestruct "HLoadRes" as (HPF) "HLoadRes". iSplitR; auto.
-           + iNext. rewrite (big_sepM_insert _ _ a (p',w)).
-             iFrame.  rewrite (big_opM_empty). all: auto.
-      - iExists ( <[a:=(p', w)]> ∅).
-        iSplitL "HLoadRes".
-        + iExists p1,g1,b1,e1,a1. iSplitR; auto.
-          case_decide; first by exfalso. auto.
-        + iNext. rewrite (big_sepM_insert _ _ a (p',w)).
-          iFrame. rewrite (big_opM_empty). all: auto.
-    }
+    iDestruct (load_res_implies_mem_map W  with "HLoadRes Ha") as (mem) "[HLoadMem HMemRes]".
 
     (* Step 3:  derive the non-spatial conditions over the memory map*)
-    iAssert (⌜mem !! a = Some (p', w)⌝ ∗ ⌜allow_load_map_or_true src (<[PC:=inr (p, g, b, e, a)]> r) mem⌝)%I with "[HLoadMem]" as %(HReadPC & HLoadAP).
-    {
-      unfold allow_load_mem_or_true.
-      iDestruct "HLoadMem" as (p1 g1 b1 e1 a1) "[% HLoadRes]".
-      unfold allow_load_map_or_true.
-      case_decide as Hallows.
-      -  pose(Hallows' := Hallows). destruct Hallows' as [Hrinr [Hra Hwb] ].
-         case_decide as Haeq.
-         * iDestruct "HLoadRes" as (p'0 w0 ->) "[% _]".
-           iSplitR. rewrite lookup_insert_ne; auto. by rewrite lookup_insert.
-           iExists p1,g1,b1,e1,a1. iSplitR; auto.
-           case_decide; last by exfalso.
-           iExists p'0,w0. iSplitR; auto.
-           by rewrite lookup_insert.
-         * iDestruct "HLoadRes" as "[-> [% HLoadRes] ]".
-           iSplitR. by rewrite lookup_insert.
-           iExists p1,g1,b1,e1,a1. iSplitR; auto.
-           case_decide; last by exfalso.
-           iExists p',w. by rewrite Haeq lookup_insert.
-      - iDestruct "HLoadRes" as "[-> HLoadRes]".
-        iSplitR. by rewrite lookup_insert.
-        iExists p1,g1,b1,e1,a1. iSplitR; auto.
-        case_decide; first by exfalso. auto.
-    }
+    iDestruct (mem_map_implies_pure_conds with "HLoadMem") as %(HReadPC & HLoadAP).
 
     (* Step 4: move the later outside, so that we can remove it after applying wp_load *)
-    iAssert (▷ allow_load_mem_or_true W src (<[PC:=inr (p, g, b, e, a)]> r) a p' w mem true)%I with "[HLoadMem]" as "HLoadMem".
-    {
-      unfold allow_load_mem_or_true.
-      iDestruct "HLoadMem" as (p0 g0 b0 e0 a0) "[% HLoadMem]".
-      do 5 (iApply later_exist_2; iExists _). iApply later_sep_2; iSplitR; auto.
-      case_decide.
-      - case_decide.
-        * iDestruct "HLoadMem" as (p'0 w0) "[-> [% HLoadMem] ]".
-        do 2 (iApply later_exist_2; iExists _).
-        do 2 (iApply later_sep_2; iSplitR; auto).
-        * iFrame.
-      - iFrame.
-    }
+    iDestruct (allow_load_mem_later with "HLoadMem") as "HLoadMem".
 
     iApply (wp_load with "[Hmap HMemRes]"); eauto.
     {by rewrite lookup_insert. }
@@ -225,52 +300,10 @@ Section fundamental.
     { subst retv.
       apply incrementPC_Some_inv in H6.
       destruct H6 as (?&?&?&?&?&?&?&?&?).
-
       iApply wp_pure_step_later; auto. iNext.
 
       (* Step 5: return all the resources we had in order to close the second location in the region, in the cases where we need to *)
-      iAssert (open_region a W ∗ a ↦ₐ[p'] w ∗ ((fixpoint interp1) W) loadv)%I with "[HLoadMem Hmem]" as "[Hr [Ha #HLVInterp ] ]".
-      {
-        unfold allow_load_mem_or_true.
-        iDestruct "HLoadMem" as (p1 g1 b1 e1 a1) "[% HLoadRes]".
-        destruct (decide (reg_allows_load (<[PC:=inr (p, g, b, e, a)]> r) src p1 g1 b1 e1 a1)). 1: rename r0 into Hallows.
-        -  destruct Hallows as [Hrinr [Hra Hwb] ].
-           destruct (decide (a1 ≠ a)); rename n into Haeq.
-           * iDestruct "HLoadRes" as (p'1 w0) "[-> [% HLoadRes] ]".
-             iDestruct "HLoadRes" as (ρ1) "(Hstate' & % & Hr & % & (Hfuture & #HV) & Hrel')".
-             iAssert ( a ↦ₐ[p'] w ∗ a1 ↦ₐ[p'1] w0)%I  with "[Hmem]" as "[$ Ha1]".
-             {
-               rewrite (big_sepM_insert); last by rewrite lookup_insert_ne.
-               rewrite (big_sepM_insert); last by auto.
-               iDestruct "Hmem" as "[Ha1 [Ha _] ]".
-               iSplitL "Ha".
-               * iDestruct "Ha" as (p2 w1 Hpair) "Ha".
-                   by inversion Hpair.
-               * iDestruct "Ha1" as (p2 w1 Hpair) "Ha".
-                   by inversion Hpair.
-             }
-             iDestruct (region_close_next with "[$Hr $Ha1 $Hrel' $Hstate' $Hfuture]") as "Hr"; eauto.
-             { apply not_elem_of_cons; split; [auto|apply not_elem_of_nil]. }
-             iDestruct (region_open_prepare with "Hr") as "$".
-             destruct H4 as (Hrinr0 & _ & _). rewrite Hrinr0 in Hrinr; inversion Hrinr.
-             rewrite H16 lookup_insert in H5; inversion H5. done.
-           * apply dec_stable in Haeq.
-             iDestruct "HLoadRes" as "[-> [% $ ] ]".
-             iAssert ( a ↦ₐ[p'] w)%I  with "[Hmem]" as "$".
-             {
-               rewrite (big_sepM_insert); last by auto.
-               iDestruct "Hmem" as "[Ha _]".
-               iDestruct "Ha" as (p2 w1 Hpair) "Ha".
-                 by inversion Hpair.
-             }
-             destruct H4 as (Hrinr0 & _ & _). rewrite Hrinr0 in Hrinr; inversion Hrinr.
-             rewrite H14 Haeq lookup_insert in H5; inversion H5. done.
-        - pose (H4' := H4).
-          destruct H4' as (Hinr0 & _ & _). destruct H8 as [Hinr1 | Hinl1].
-          * rewrite Hinr0 in Hinr1. inversion Hinr1.
-            rewrite H9 H10 H11 H12 H13 in H4. by exfalso.
-          * destruct Hinl1 as [z Hinl1]. rewrite Hinl1 in Hinr0. by exfalso.
-      }
+      iDestruct (mem_map_recover_res with "HLoadMem Hw Hmem") as "[Hr [Ha #HLVInterp ] ]"; eauto.
 
       (* Exceptional success case: we do not apply the induction hypothesis in case we have a faulty PC*)
       destruct (decide (x = RX ∨ x = RWX ∨ x = RWLX)).
